restructured the project, mem_imp, mem_spec, proof done for n bit bus signals.

src/Sequential.lean
@@ -1,11 +1,33 @@
-import Gates tactic 
+import Gates tactic Conversions
 
-def clk : ℕ → bool
-| 0 := tt
-| (n+1) := if clk n then ff else tt
+def stream (α : Type) := ℕ → α
 
-def test_clk : ℕ → list bool
-| 0 := [clk 0]
-| (n+1) := (clk (n+1)) :: test_clk n
+def signal := ℕ → bool
 
-#eval test_clk 10 
+def sig_n (n : ℕ) := ℕ → array n bool
+
+def mem_imp (I: bool) (D S: signal) : signal
+| nat.zero := I
+| (nat.succ y) := if S y = tt then D y 
+                  else mem_imp y
+
+def mem_spec (D S M: signal): Prop :=
+  ∀ t : ℕ,
+    (S t = tt → M (nat.succ t) = D t) ∧ --frame 1 D S M+1
+    (S t = ff → M (nat.succ t) = M t) --frame 2 S M M+1
+
+def n_mem_imp {n : ℕ} (I : array n bool) (D : sig_n n) (S : signal) : sig_n n
+  | nat.zero := I
+  | (nat.succ y) := if S y = tt then D y
+                    else n_mem_imp y
+
+def n_mem_spec {n : ℕ} (D : sig_n n) (S : signal) (M: sig_n n): Prop :=
+  ∀ t : ℕ,
+    (S t = tt → M (nat.succ t) = D t) ∧  --frame 1 D S M+1
+    ( S t = ff → M (nat.succ t) = M t) --frame 2 S M M+1
+
+def ncounter_spec {n : ℕ} (out : sig_n n) (res : signal) : Prop :=
+  ∀ t : ℕ, 
+  if res t = tt 
+  then bool_arr_to_nat(out (t+1)) = 0
+  else bool_arr_to_nat(out (t+1)) = (bool_arr_to_nat(out t) + 1) % 2^(n)
