src/Combinational.lean
@@ -1,0 +1,19 @@
+import Gates tactic Conversions data.vector data.real.basic
+
+def mux_imp (in1 in2 sel out : bool) : Prop :=
+	∃ (p q r : bool), (nand_n [in1, p] q) ∧ (nand_n [sel, in2] r) ∧ 
+		(nand_n [q, r] out) ∧ (not_ sel p)
+
+def mux_spec (in1 in2 sel out : bool) : Prop :=
+	if sel then (out = in2) else (out = in1) 
+
+def dec_imp (in0 in1 out0 out1 out2 out3 : bool) : Prop :=
+	∃ (p q : bool), (not_ in0 p) ∧ (not_ in1 q) ∧ (and_n [p, q] out0) ∧ 
+		(and_n [in0, q] out1) ∧ (and_n [p, in1] out2) ∧ (and_n [in0, in1] out3)
+
+def dec_spec (in0 in1 out0 out1 out2 out3 : bool) : Prop :=
+	if ¬in1 ∧ ¬in0 then (out3 = ff ∧ out2 = ff ∧ out1 = ff ∧ out0 = tt)
+	else if ¬in1 ∧ in0 then (out3 = ff ∧ out2 = ff ∧ out1 = tt ∧ out0 = ff)
+	else if in1 ∧ ¬in0 then (out3 = ff ∧ out2 = tt ∧ out1 = ff ∧ out0 = ff)
+	else (out3 = tt ∧ out2 = ff ∧ out1 = ff ∧ out0 = ff)
+
