src/Conversions.lean
@@ -7,3 +7,24 @@ def bool_list_to_nat : list bool → ℕ
 
 def bool_vec_to_nat {n : ℕ} (v : vector bool n) : ℕ :=
   bool_list_to_nat (list.of_fn v.nth)
+
+def bool_arr_to_nat {n : ℕ} (v : array n bool) : ℕ :=
+  bool_list_to_nat (array.to_list v)
+
+def get_nth_bool : list bool -> ℕ -> bool
+  | [] n := ff
+  | (h::t) 0 := h
+  | (h::t) (n+1) := get_nth_bool t n
+
+def get_first_half {α : Type*} : list α → list α --Type* is Type 0, smallest universe, non dependent types
+  | [] := []
+  | [a] := [a]
+  | lst := list.take (lst.length / 2) lst
+
+def get_second_half {α : Type*} : list α → list α
+  | [] := []
+  | [a] := [a]
+  | lst := list.drop (lst.length / 2) lst
+
+#eval get_first_half [tt, tt, ff, tt, ff, tt, ff]
+#eval get_second_half [tt, tt, ff, tt, ff, tt, ff]
