src/Lemmas.lean
@@ -1,0 +1,129 @@
+import Sequential Combinational
+
+lemma mem_imp_complies_to_spec (D S: signal) :
+  mem_spec D S (mem_imp ff D S) :=
+  begin
+    unfold mem_spec,
+    intro t,
+    split,
+    {
+      intros h,
+      unfold mem_imp,
+      simp,
+      intro h',
+      exfalso,
+      rewrite h at h',
+      simp at h',
+      assumption,
+    },
+    {
+      intros h,
+      unfold mem_imp,
+      simp,
+      intro h',
+      exfalso,
+      rewrite h at h',
+      simp at h',
+      assumption,
+    }
+  end
+
+lemma n_mem_imp_complies_to_spec {n : ℕ} (D : sig_n n) (S: signal):
+  n_mem_spec D S (n_mem_imp (mk_array n ff) D S) :=
+  begin
+    unfold n_mem_spec,
+    intros t,
+    split,
+    {
+      intros h,
+      unfold n_mem_imp,
+      simp,
+      intro h',
+      exfalso,
+      rewrite h at h',
+      simp at h',
+      assumption,
+    },
+    {
+      intros h,
+      unfold n_mem_imp,
+      simp,
+      intro h',
+      exfalso,
+      rewrite h at h',
+      simp at h',
+      assumption,
+    }
+  end
+
+lemma mux_correct : ∀ in1 in2 sel out, mux_imp in1 in2 sel out ↔ mux_spec in1 in2 sel out :=
+begin
+  intros in1 in2 sel out,
+  unfold mux_imp mux_spec nand_n AND not_,
+  split,
+  {
+    cases sel; simp,
+    { --sel FF
+      cases in1; simp,
+    },
+    { --sel TT
+      cases in2; simp,
+    }
+  },
+  {
+    cases sel; simp,
+    {
+      cases in1; simp,
+    },
+    { 
+      cases in2; simp,
+    }
+  }
+end
+
+theorem dec_correct : ∀ in0 in1 out0 out1 out2 out3, 
+			dec_imp in0 in1 out0 out1 out2 out3 ↔ dec_spec in0 in1 out0 out1 out2 out3 :=
+begin
+  intros in0 in1 out0 out1 out2 out3,
+  unfold dec_imp dec_spec not_ and_n AND,
+  simp,
+  split,
+  {
+    cases in0; cases in1; simp *,
+    {
+      intros a b c d,
+      cases a; cases b; cases c; cases d; simp,
+    },
+    {
+      intros a b c d,
+      cases a; cases b; cases c; cases d; simp,
+    },
+    {
+      intros a b c d,
+      cases a; cases b; cases c; cases d; simp,
+    },
+    {
+      intros a b c d,
+      cases a; cases b; cases c; cases d; simp,
+    }
+  },
+  {
+    cases in0; cases in1; simp *,
+    {
+      intros a b c d,
+      cases a; cases b; cases c; cases d; simp,
+    },
+    {
+      intros a b c d,
+      cases a; cases b; cases c; cases d; simp,
+    },
+    {
+      intros a b c d,
+      cases a; cases b; cases c; cases d; simp,
+    },
+    {
+      intros a b c d,
+      cases a; cases b; cases c; cases d; simp,
+    }
+  }
+end
